feat: improve support for equations in cutsat (#7203)
This PR improves the support for equalities in cutsat. It also
simplifies a few support theorems used to justify cutsat rules.

src/Init/Data/Int/Linear.lean
@@ -850,6 +850,12 @@ theorem le_unsat (ctx : Context) (p : Poly) : p.isUnsatLe → p.denote' ctx ≤ 
   have := Int.lt_of_le_of_lt h₂ h₁
   simp at this
 
+theorem eq_norm (ctx : Context) (p₁ p₂ : Poly) (h : p₁.norm == p₂) : p₁.denote' ctx = 0 → p₂.denote' ctx = 0 := by
+  simp at h
+  replace h := congrArg (Poly.denote ctx) h
+  simp at h
+  simp [*]
+
 def Poly.coeff (p : Poly) (x : Var) : Int :=
   match p with
   | .add a y p => bif x == y then a else coeff p x
@@ -864,17 +870,28 @@ private theorem dvd_of_eq' {a x p : Int} : a*x + p = 0 → a ∣ p := by
   rw [Int.mul_comm, ← Int.neg_mul, Eq.comm, Int.mul_comm] at h
   exact ⟨-x, h⟩
 
+private def abs (x : Int) : Int :=
+  Int.ofNat x.natAbs
+
+private theorem abs_dvd {a p : Int} (h : a ∣ p) : abs a ∣ p := by
+  cases a <;> simp [abs]
+  · simp at h; assumption
+  · simp [Int.negSucc_eq] at h; assumption
+
 def dvd_of_eq_cert (x : Var) (p₁ : Poly) (d₂ : Int) (p₂ : Poly) : Bool :=
-  d₂ == p₁.coeff x && p₂ == p₁.insert (-d₂) x
+  let a := p₁.coeff x
+  d₂ == abs a && p₂ == p₁.insert (-a) x
 
 theorem dvd_of_eq (ctx : Context) (x : Var) (p₁ : Poly) (d₂ : Int) (p₂ : Poly)
     : dvd_of_eq_cert x p₁ d₂ p₂ → p₁.denote' ctx = 0 → d₂ ∣ p₂.denote' ctx := by
   simp [dvd_of_eq_cert]
   intro h₁ h₂
   have h := eq_add_coeff_insert ctx p₁ x
-  rw [← h₁, ← h₂] at h
-  rw [h]
-  apply dvd_of_eq'
+  rw [← h₂] at h
+  rw [h, h₁]
+  intro h₃
+  apply abs_dvd
+  apply dvd_of_eq' h₃
 
 private theorem eq_dvd_subst' {a x p d b q : Int} : a*x + p = 0 → d ∣ b*x + q → a*d ∣ a*q - b*p := by
   intro h₁ ⟨z, h₂⟩
@@ -892,7 +909,7 @@ def eq_dvd_subst_cert (x : Var) (p₁ : Poly) (d₂ : Int) (p₂ : Poly) (d₃ :
   let b := p₂.coeff x
   let p := p₁.insert (-a) x
   let q := p₂.insert (-b) x
-  d₃ == a * d₂ &&
+  d₃ == abs (a * d₂) &&
   p₃ == (q.mul a |>.combine (p.mul (-b)))
 
 theorem eq_dvd_subst (ctx : Context) (x : Var) (p₁ : Poly) (d₂ : Int) (p₂ : Poly) (d₃ : Int) (p₃ : Poly)
@@ -913,124 +930,53 @@ theorem eq_dvd_subst (ctx : Context) (x : Var) (p₁ : Poly) (d₂ : Int) (p₂ 
   rw [Int.add_comm] at h₁ h₂
   have := eq_dvd_subst' h₁ h₂
   rw [Int.sub_eq_add_neg, Int.add_comm] at this
+  apply abs_dvd
   simp [this]
-
-private theorem eq_eq_subst' {a x p b q : Int} : a*x + p = 0 → b*x + q = 0 → b*p - a*q = 0 := by
-  intro h₁ h₂
-  replace h₁ := congrArg (b*·) h₁; simp at h₁
-  replace h₂ := congrArg ((-a)*.) h₂; simp at h₂
-  rw [Int.add_comm] at h₁
-  replace h₁ := Int.neg_eq_of_add_eq_zero h₁
-  rw [← h₁]; clear h₁
-  replace h₂ := Int.neg_eq_of_add_eq_zero h₂; simp at h₂
-  rw [h₂]; clear h₂
-  rw [Int.mul_left_comm]
-  simp
 
 def eq_eq_subst_cert (x : Var) (p₁ : Poly) (p₂ : Poly) (p₃ : Poly) : Bool :=
   let a := p₁.coeff x
   let b := p₂.coeff x
-  let p := p₁.insert (-a) x
-  let q := p₂.insert (-b) x
-  p₃ == (p.mul b |>.combine (q.mul (-a)))
+  p₃ == (p₁.mul b |>.combine (p₂.mul (-a)))
 
 theorem eq_eq_subst (ctx : Context) (x : Var) (p₁ : Poly) (p₂ : Poly) (p₃ : Poly)
     : eq_eq_subst_cert x p₁ p₂ p₃ → p₁.denote' ctx = 0 → p₂.denote' ctx = 0 → p₃.denote' ctx = 0 := by
   simp [eq_eq_subst_cert]
-  have eq₁ := eq_add_coeff_insert ctx p₁ x
-  have eq₂ := eq_add_coeff_insert ctx p₂ x
-  revert eq₁ eq₂
-  generalize p₁.coeff x = a
-  generalize p₂.coeff x = b
-  generalize p₁.insert (-a) x = p
-  generalize p₂.insert (-b) x = q
-  intro eq₁; simp [eq₁]; clear eq₁
-  intro eq₂; simp [eq₂]; clear eq₂
   intro; subst p₃
   intro h₁ h₂
-  rw [Int.add_comm] at h₁ h₂
-  have := eq_eq_subst' h₁ h₂
-  rw [Int.sub_eq_add_neg] at this
-  simp [this]
-
-private theorem eq_le_subst_nonneg' {a x p b q : Int} : a ≥ 0 → a*x + p = 0 → b*x + q ≤ 0 → a*q - b*p ≤ 0 := by
-  intro h h₁ h₂
-  replace h₁ := congrArg ((-b)*·) h₁; simp at h₁
-  rw [Int.add_comm, Int.mul_left_comm] at h₁
-  replace h₁ := Int.neg_eq_of_add_eq_zero h₁; simp at h₁
-  replace h₂ := Int.mul_le_mul_of_nonneg_left h₂ h
-  rw [Int.mul_add, h₁] at h₂; clear h₁
-  simp at h₂
-  rw [Int.sub_eq_add_neg]
-  assumption
+  simp [*]
 
 def eq_le_subst_nonneg_cert (x : Var) (p₁ : Poly) (p₂ : Poly) (p₃ : Poly) : Bool :=
   let a := p₁.coeff x
   let b := p₂.coeff x
-  let p := p₁.insert (-a) x
-  let q := p₂.insert (-b) x
-  a ≥ 0 && p₃ == (q.mul a |>.combine (p.mul (-b)))
+  a ≥ 0 && p₃ == (p₂.mul a |>.combine (p₁.mul (-b)))
 
 theorem eq_le_subst_nonneg (ctx : Context) (x : Var) (p₁ : Poly) (p₂ : Poly) (p₃ : Poly)
     : eq_le_subst_nonneg_cert x p₁ p₂ p₃ → p₁.denote' ctx = 0 → p₂.denote' ctx ≤ 0 → p₃.denote' ctx ≤ 0 := by
   simp [eq_le_subst_nonneg_cert]
-  have eq₁ := eq_add_coeff_insert ctx p₁ x
-  have eq₂ := eq_add_coeff_insert ctx p₂ x
-  revert eq₁ eq₂
-  generalize p₁.coeff x = a
-  generalize p₂.coeff x = b
-  generalize p₁.insert (-a) x = p
-  generalize p₂.insert (-b) x = q
-  intro eq₁; simp [eq₁]; clear eq₁
-  intro eq₂; simp [eq₂]; clear eq₂
   intro h
   intro; subst p₃
   intro h₁ h₂
-  rw [Int.add_comm] at h₁ h₂
-  have := eq_le_subst_nonneg' h h₁ h₂
-  rw [Int.sub_eq_add_neg, Int.add_comm] at this
-  simp [this]
-
-private theorem eq_le_subst_nonpos' {a x p b q : Int} : a ≤ 0 → a*x + p = 0 → b*x + q ≤ 0 → b*p - a*q ≤ 0 := by
-  intro h h₁ h₂
-  replace h₁ := congrArg (b*·) h₁; simp at h₁
-  rw [Int.add_comm, Int.mul_left_comm] at h₁
-  replace h₁ := Int.neg_eq_of_add_eq_zero h₁; simp at h₁
-  replace h : (-a) ≥ 0 := by
-    have := Int.neg_le_neg h
-    simp at this
-    exact this
-  replace h₂ := Int.mul_le_mul_of_nonneg_left h₂ h; simp at h₂; clear h
-  rw [h₁] at h₂
-  rw [Int.add_comm, ←Int.sub_eq_add_neg] at h₂
-  assumption
+  replace h₂ := Int.mul_le_mul_of_nonneg_left h₂ h
+  simp at h₂
+  simp [*]
 
 def eq_le_subst_nonpos_cert (x : Var) (p₁ : Poly) (p₂ : Poly) (p₃ : Poly) : Bool :=
   let a := p₁.coeff x
   let b := p₂.coeff x
-  let p := p₁.insert (-a) x
-  let q := p₂.insert (-b) x
-  a ≤ 0 && p₃ == (p.mul b |>.combine (q.mul (-a)))
+  a ≤ 0 && p₃ == (p₁.mul b |>.combine (p₂.mul (-a)))
 
 theorem eq_le_subst_nonpos (ctx : Context) (x : Var) (p₁ : Poly) (p₂ : Poly) (p₃ : Poly)
     : eq_le_subst_nonpos_cert x p₁ p₂ p₃ → p₁.denote' ctx = 0 → p₂.denote' ctx ≤ 0 → p₃.denote' ctx ≤ 0 := by
   simp [eq_le_subst_nonpos_cert]
-  have eq₁ := eq_add_coeff_insert ctx p₁ x
-  have eq₂ := eq_add_coeff_insert ctx p₂ x
-  revert eq₁ eq₂
-  generalize p₁.coeff x = a
-  generalize p₂.coeff x = b
-  generalize p₁.insert (-a) x = p
-  generalize p₂.insert (-b) x = q
-  intro eq₁; simp [eq₁]; clear eq₁
-  intro eq₂; simp [eq₂]; clear eq₂
   intro h
   intro; subst p₃
   intro h₁ h₂
-  rw [Int.add_comm] at h₁ h₂
-  have := eq_le_subst_nonpos' h h₁ h₂
-  rw [Int.sub_eq_add_neg] at this
-  simp [this]
+  simp [*]
+  replace h₂ := Int.mul_le_mul_of_nonpos_left h₂ h; simp at h₂; clear h
+  rw [← Int.neg_zero]
+  apply Int.neg_le_neg
+  rw [Int.mul_comm]
+  assumption
 
 end Int.Linear
 
