src/Lean/Meta/Tactic/Grind/Arith/Cutsat/EqCnstr.lean
@@ -5,10 +5,79 @@ Authors: Leonardo de Moura
 -/
 prelude
 import Lean.Meta.Tactic.Grind.Arith.Cutsat.Var
+import Lean.Meta.Tactic.Grind.Arith.Cutsat.DvdCnstr
 
 namespace Lean.Meta.Grind.Arith.Cutsat
+
 def mkEqCnstr (p : Poly) (h : EqCnstrProof) : GoalM EqCnstr := do
   return { p, h, id := (← mkCnstrId) }
+
+def EqCnstr.norm (c : EqCnstr) : GoalM EqCnstr := do
+  let c ← if c.p.isSorted then
+    pure c
+  else
+    mkEqCnstr c.p.norm (.norm c)
+
+/--
+Selects the variable in the given linear polynomial whose coefficient has the smallest absolute value.
+-/
+def _root_.Int.Linear.Poly.pickVarToElim? (p : Poly) : Option (Int × Var) :=
+  match p with
+  | .num _ => none
+  | .add k x p => go k x p
+where
+  go (k : Int) (x : Var) (p : Poly) : Int × Var :=
+    if k == 1 || k == -1 then
+      (k, x)
+    else match p with
+      | .num _ => (k, x)
+      | .add k' x' p =>
+        if k'.natAbs < k.natAbs then
+          go k' x' p
+        else
+          go k x p
+
+/--
+Given a polynomial `p`, returns `some (x, k, c)` if `p` contains the monomial `k*x`,
+and `x` has been eliminated using the equality `c`.
+-/
+def _root_.Int.Linear.Poly.findVarToSubst (p : Poly) : GoalM (Option (Int × Var × EqCnstr)) := do
+  match p with
+  | .num _ => return none
+  | .add k x p =>
+    if let some c := (← get').elimEqs[x]! then
+      return some (k, x, c)
+    else
+      findVarToSubst p
+
+partial def applySubsts (c : EqCnstr) : GoalM EqCnstr := do
+  let some (a, x, c₁) ← c.p.findVarToSubst | return c
+  trace[grind.cutsat.subst] "{← getVar x}, {← c.pp}, {← c₁.pp}"
+  let b := c₁.p.coeff x
+  let p := c.p.mul (-b) |>.combine (c₁.p.mul a)
+  let c ← mkEqCnstr p (.subst x c₁ c)
+  applySubsts c
+
+def EqCnstr.assert (c : EqCnstr) : GoalM Unit := do
+  if (← isInconsistent) then return ()
+  trace[grind.cutsat.assert] "{← c.pp}"
+  let c ← c.norm
+  let c ← applySubsts c
+  -- TODO: check coeffsr
+  trace[grind.cutsat.eq] "{← c.pp}"
+  let some (k, x) := c.p.pickVarToElim? | c.throwUnexpected
+  -- TODO: eliminate `x` from lowers, uppers, and dvdCnstrs
+  -- TODO: reset `x`s occurrences
+  -- assert a divisibility constraint IF `|k| != 1`
+  if k.natAbs != 1 then
+    let p := c.p.insert (-k) x
+    let d := Int.ofNat k.natAbs
+    let c ← mkDvdCnstr d p (.ofEq x c)
+    c.assert
+  modify' fun s => { s with
+    elimEqs := s.elimEqs.set x (some c)
+    elimStack := x :: s.elimStack
+  }
 
 @[export lean_process_cutsat_eq]
 def processNewEqImpl (a b : Expr) : GoalM Unit := do
@@ -17,10 +86,14 @@ def processNewEqImpl (a b : Expr) : GoalM Unit := do
   return ()
 
 @[export lean_process_new_cutsat_lit]
-def processNewEqLitImpl (a k : Expr) : GoalM Unit := do
-  trace[grind.cutsat.eq] "{mkIntEq a k}"
-  -- TODO
-  return ()
+def processNewEqLitImpl (a ke : Expr) : GoalM Unit := do
+  let some k ← getIntValue? ke | return ()
+  let some p := (← get').terms.find? { expr := a } | return ()
+  if k == 0 then
+    (← mkEqCnstr p (.expr (← mkEqProof a ke))).assert
+  else
+    -- TODO
+    return ()
 
 /-- Different kinds of terms internalized by this module. -/
 private inductive SupportedTermKind where
