src/Lean/Meta/Tactic/Grind/Arith/Cutsat.lean
@@ -18,6 +18,7 @@ import Lean.Meta.Tactic.Grind.Arith.Cutsat.EqCnstr
 namespace Lean
 
 builtin_initialize registerTraceClass `grind.cutsat
+builtin_initialize registerTraceClass `grind.cutsat.subst
 builtin_initialize registerTraceClass `grind.cutsat.eq
 builtin_initialize registerTraceClass `grind.cutsat.assert
 builtin_initialize registerTraceClass `grind.cutsat.assert.dvd
